complete proof

messageInvariantPrototypes/toyLeaderElection/monotonic_no-recv-send_option-nominee/applicationProof.dfy
@@ -14,13 +14,16 @@ import opened Obligations
 *                                Application Invariants                                *
 ***************************************************************************************/
 
-// Application Invariant: requires message invariants to be inductive
-// Compared to the version without Monotonic Transformation, we now only talk about host state
-ghost predicate VotersVoteOnce(c: Constants, v: Variables) 
+// Application Invariant: Host having a vote implies voter nominated that host
+ghost predicate HasVoteImpliesVoterNominates(c: Constants, v: Variables)
   requires v.WF(c)
 {
-  forall idx | c.ValidIdx(idx)
-  :: |v.hosts[idx].nominee| <= 1
+  forall nominee, voter | 
+    && c.ValidIdx(nominee)
+    && c.ValidIdx(voter)
+    && v.hosts[nominee].HasVoteFrom(voter)
+  ::
+    v.hosts[voter].Nominates(nominee)
 }
 
 // Application bundle
@@ -28,7 +31,7 @@ ghost predicate ApplicationInv(c: Constants, v: Variables)
   requires v.WF(c)
   requires MessageInv(c, v)
 {
-  VotersVoteOnce(c, v)
+  HasVoteImpliesVoterNominates(c, v)
 }
 
 ghost predicate Inv(c: Constants, v: Variables)
@@ -64,7 +67,7 @@ lemma InvInductive(c: Constants, v: Variables, v': Variables)
 
 lemma SafetyProof(c: Constants, v: Variables) 
   requires MessageInv(c, v)
-  requires VotersVoteOnce(c, v)
+  requires HasVoteImpliesVoterNominates(c, v)
   ensures Safety(c, v)
 {
   /* Proof by contradiction: Assume two leaders were elected in v', L1 and L2.
